examples/ghc/lib/Exitify.v
@@ -14,13 +14,20 @@ Require Coq.Program.Wf.
 
 Require AxiomatizedTypes.
 Require BasicTypes.
+Require Coq.Init.Datatypes.
+Require Coq.Lists.List.
 Require Core.
+Require CoreFVs.
 Require CoreUtils.
 Require Data.Bifunctor.
 Require Data.Foldable.
+Require Data.Traversable.
 Require Data.Tuple.
 Require GHC.Base.
+Require GHC.Err.
+Require GHC.Prim.
 Require GHC.Utils.Monad.State.Strict.
+Require HsToCoq.DeferredFix.
 Require Id.
 Require Util.
 Import GHC.Base.Notations.
@@ -33,8 +40,184 @@ Import GHC.Base.Notations.
 
 (* Converted value declarations: *)
 
-Axiom exitifyRec : Core.InScopeSet ->
-                   list (Core.Var * Core.CoreExpr)%type -> list Core.CoreBind.
+Axiom mkExitJoinId : Core.InScopeSet ->
+                     AxiomatizedTypes.Type_ -> BasicTypes.JoinArity -> ExitifyM Core.JoinId.
+
+#[global] Definition addExit
+   : Core.InScopeSet ->
+     BasicTypes.JoinArity -> Core.CoreExpr -> ExitifyM Core.JoinId :=
+  fun in_scope join_arity rhs =>
+    let ty := CoreUtils.exprType rhs in
+    mkExitJoinId in_scope ty join_arity GHC.Base.>>=
+    (fun v =>
+       GHC.Utils.Monad.State.Strict.get GHC.Base.>>=
+       (fun fs =>
+          GHC.Utils.Monad.State.Strict.put (cons (pair v rhs) fs) GHC.Base.>>
+          GHC.Base.return_ v)).
+
+#[global] Definition exitifyRec
+   : Core.InScopeSet ->
+     list (Core.Var * Core.CoreExpr)%type -> list Core.CoreBind :=
+  fun in_scope pairs =>
+    let go_exit
+     : list Core.Var -> Core.CoreExpr -> Core.VarSet -> ExitifyM Core.CoreExpr :=
+      fun captured e fvs =>
+        let zap :=
+          fun v => if Core.isId v : bool then Id.setIdInfo v Core.vanillaIdInfo else v in
+        let abs_vars :=
+          let pick :=
+            fun arg_1__ arg_2__ =>
+              match arg_1__, arg_2__ with
+              | v, pair fvs' acc =>
+                  if Core.elemVarSet v fvs' : bool
+                  then pair (Core.delVarSet fvs' v) (cons (zap v) acc) else
+                  pair fvs' acc
+              end in
+          Data.Tuple.snd (Data.Foldable.foldr pick (pair fvs nil) captured) in
+        let captures_join_points := Data.Foldable.any Id.isJoinId abs_vars in
+        let is_interesting :=
+          Core.anyVarSet Core.isLocalId (Core.minusVarSet fvs (Core.mkVarSet captured)) in
+        let isCapturedVarArg :=
+          fun arg_9__ =>
+            match arg_9__ with
+            | Core.Mk_Var v => Data.Foldable.elem v captured
+            | _ => false
+            end in
+        let j_14__ :=
+          let avoid := Core.extendInScopeSetList in_scope captured in
+          let rhs := Core.mkLams abs_vars e in
+          addExit avoid (Coq.Lists.List.length abs_vars) rhs GHC.Base.>>=
+          (fun v => GHC.Base.return_ (Core.mkVarApps (Core.Mk_Var v) abs_vars)) in
+        let j_15__ :=
+          if captures_join_points : bool then GHC.Base.return_ e else
+          j_14__ in
+        let j_16__ :=
+          if negb is_interesting : bool then GHC.Base.return_ e else
+          j_15__ in
+        match Core.collectArgs e with
+        | pair (Core.Mk_Var f) args =>
+            if andb (Id.isJoinId f) (Data.Foldable.all isCapturedVarArg args) : bool
+            then GHC.Base.return_ e else
+            j_16__
+        | _ => j_16__
+        end in
+    let recursive_calls := Core.mkVarSet (GHC.Base.map Data.Tuple.fst pairs) in
+    let go : list Core.Var -> CoreFVs.CoreExprWithFVs -> ExitifyM Core.CoreExpr :=
+      HsToCoq.DeferredFix.deferredFix2 (fun go
+                                        (arg_19__ : list Core.Var)
+                                        (arg_20__ : CoreFVs.CoreExprWithFVs) =>
+                                          match arg_19__, arg_20__ with
+                                          | captured, ann_e =>
+                                              let j_22__ :=
+                                                match arg_19__, arg_20__ with
+                                                | _, ann_e => GHC.Base.return_ (Core.deAnnotate ann_e)
+                                                end in
+                                              let j_40__ :=
+                                                match arg_19__, arg_20__ with
+                                                | captured, pair _ (Core.AnnCase scrut bndr ty alts) =>
+                                                    Data.Traversable.forM alts (fun '(Core.Mk_AnnAlt dc pats rhs) =>
+                                                                                  go (Coq.Init.Datatypes.app captured
+                                                                                                             (Coq.Init.Datatypes.app
+                                                                                                              (cons bndr
+                                                                                                                    nil)
+                                                                                                              pats)) rhs
+                                                                                  GHC.Base.>>=
+                                                                                  (fun rhs' =>
+                                                                                     GHC.Base.return_ (Core.Mk_Alt dc
+                                                                                                       pats rhs')))
+                                                    GHC.Base.>>=
+                                                    (fun alts' =>
+                                                       GHC.Base.return_ (Core.Case (Core.deAnnotate scrut) bndr ty
+                                                                                   alts'))
+                                                | captured, pair _ (Core.AnnLet ann_bind body) =>
+                                                    let bind := Core.deAnnBind ann_bind in
+                                                    let j_37__ :=
+                                                      go (Coq.Init.Datatypes.app captured (Core.bindersOf bind)) body
+                                                      GHC.Base.>>=
+                                                      (fun body' => GHC.Base.return_ (Core.Let bind body')) in
+                                                    let j_38__ :=
+                                                      match ann_bind with
+                                                      | Core.AnnRec pairs =>
+                                                          if Id.isJoinId (Data.Tuple.fst (GHC.Err.head pairs)) : bool
+                                                          then let js := GHC.Base.map Data.Tuple.fst pairs in
+                                                               Data.Traversable.forM pairs (fun '(pair j rhs) =>
+                                                                                              let join_arity :=
+                                                                                                Id.idJoinArity j in
+                                                                                              let 'pair params
+                                                                                                 join_body :=
+                                                                                                Core.collectNAnnBndrs
+                                                                                                  join_arity rhs in
+                                                                                              go (Coq.Init.Datatypes.app
+                                                                                                  captured
+                                                                                                  (Coq.Init.Datatypes.app
+                                                                                                   js params)) join_body
+                                                                                              GHC.Base.>>=
+                                                                                              (fun join_body' =>
+                                                                                                 let rhs' :=
+                                                                                                   Core.mkLams params
+                                                                                                   join_body' in
+                                                                                                 GHC.Base.return_ (pair
+                                                                                                                   j
+                                                                                                                   rhs')))
+                                                               GHC.Base.>>=
+                                                               (fun pairs' =>
+                                                                  go (Coq.Init.Datatypes.app captured js) body
+                                                                  GHC.Base.>>=
+                                                                  (fun body' =>
+                                                                     GHC.Base.return_ (Core.Let (Core.Rec pairs')
+                                                                                                body'))) else
+                                                          j_37__
+                                                      | _ => j_37__
+                                                      end in
+                                                    match ann_bind with
+                                                    | Core.AnnNonRec j rhs =>
+                                                        match Id.idJoinPointHood j with
+                                                        | Outputable.JoinPoint join_arity =>
+                                                            let 'pair params join_body := Core.collectNAnnBndrs
+                                                                                            join_arity rhs in
+                                                            go (Coq.Init.Datatypes.app captured params) join_body
+                                                            GHC.Base.>>=
+                                                            (fun join_body' =>
+                                                               let rhs' := Core.mkLams params join_body' in
+                                                               go (Coq.Init.Datatypes.app captured (cons j nil)) body
+                                                               GHC.Base.>>=
+                                                               (fun body' =>
+                                                                  GHC.Base.return_ (Core.Let (Core.NonRec j rhs')
+                                                                                             body')))
+                                                        | _ => j_38__
+                                                        end
+                                                    | _ => j_38__
+                                                    end
+                                                | _, _ => j_22__
+                                                end in
+                                              let fvs :=
+                                                Core.dVarSetToVarSet (CoreFVs.exprFreeVars (Core.deAnnotate ann_e)) in
+                                              if Core.disjointVarSet fvs recursive_calls : bool
+                                              then go_exit captured (Core.deAnnotate ann_e) fvs else
+                                              j_40__
+                                          end) in
+    let ann_pairs := GHC.Base.map (Data.Bifunctor.second CoreFVs.freeVars) pairs in
+    let 'pair pairs' exits := GHC.Prim.rightSection
+                                GHC.Utils.Monad.State.Strict.runState nil (Data.Traversable.forM ann_pairs
+                                                                                                 (fun '(pair x rhs) =>
+                                                                                                    let 'pair args
+                                                                                                       body :=
+                                                                                                      Core.collectNAnnBndrs
+                                                                                                        (Id.idJoinArity
+                                                                                                         x) rhs in
+                                                                                                    go args body
+                                                                                                    GHC.Base.>>=
+                                                                                                    (fun body' =>
+                                                                                                       let rhs' :=
+                                                                                                         Core.mkLams
+                                                                                                         args body' in
+                                                                                                       GHC.Base.return_
+                                                                                                       (pair x
+                                                                                                             rhs')))) in
+    Coq.Init.Datatypes.app (let cont_51__ arg_52__ :=
+                              let 'pair xid rhs := arg_52__ in
+                              cons (Core.NonRec xid rhs) nil in
+                            Coq.Lists.List.flat_map cont_51__ exits) (cons (Core.Rec pairs') nil).
 
 #[global] Definition exitifyProgram : Core.CoreProgram -> Core.CoreProgram :=
   fun binds =>
@@ -80,30 +263,27 @@ Axiom exitifyRec : Core.InScopeSet ->
         end in
     GHC.Base.map goTopLvl binds.
 
-Axiom mkExitJoinId : Core.InScopeSet ->
-                     AxiomatizedTypes.Type_ -> BasicTypes.JoinArity -> ExitifyM Core.JoinId.
-
-#[global] Definition addExit
-   : Core.InScopeSet ->
-     BasicTypes.JoinArity -> Core.CoreExpr -> ExitifyM Core.JoinId :=
-  fun in_scope join_arity rhs =>
-    let ty := CoreUtils.exprType rhs in
-    mkExitJoinId in_scope ty join_arity GHC.Base.>>=
-    (fun v =>
-       GHC.Utils.Monad.State.Strict.get GHC.Base.>>=
-       (fun fs =>
-          GHC.Utils.Monad.State.Strict.put (cons (pair v rhs) fs) GHC.Base.>>
-          GHC.Base.return_ v)).
-
 (* External variables:
-     bool cons list op_zt__ pair AxiomatizedTypes.Type_ BasicTypes.JoinArity Core.App
-     Core.Case Core.Cast Core.CoreBind Core.CoreExpr Core.CoreProgram Core.InScopeSet
-     Core.JoinId Core.Lam Core.Let Core.Lit Core.Mk_Alt Core.Mk_Coercion Core.Mk_Type
-     Core.Mk_Var Core.NonRec Core.Rec Core.Var Core.emptyInScopeSet
-     Core.extendInScopeSet Core.extendInScopeSetList Core.mkLets CoreUtils.exprType
-     CoreUtils.extendInScopeSetBind CoreUtils.extendInScopeSetBndrs
-     Data.Bifunctor.second Data.Foldable.any Data.Tuple.fst GHC.Base.map
-     GHC.Base.op_z2218U__ GHC.Base.op_zgzg__ GHC.Base.op_zgzgze__ GHC.Base.return_
-     GHC.Utils.Monad.State.Strict.State GHC.Utils.Monad.State.Strict.get
-     GHC.Utils.Monad.State.Strict.put Id.isJoinId Util.mapSnd
+     andb bool cons false list negb nil op_zt__ pair AxiomatizedTypes.Type_
+     BasicTypes.JoinArity Coq.Init.Datatypes.app Coq.Lists.List.flat_map
+     Coq.Lists.List.length Core.AnnCase Core.AnnLet Core.AnnNonRec Core.AnnRec
+     Core.App Core.Case Core.Cast Core.CoreBind Core.CoreExpr Core.CoreProgram
+     Core.InScopeSet Core.JoinId Core.Lam Core.Let Core.Lit Core.Mk_Alt
+     Core.Mk_AnnAlt Core.Mk_Coercion Core.Mk_Type Core.Mk_Var Core.NonRec Core.Rec
+     Core.Var Core.VarSet Core.anyVarSet Core.bindersOf Core.collectArgs
+     Core.collectNAnnBndrs Core.dVarSetToVarSet Core.deAnnBind Core.deAnnotate
+     Core.delVarSet Core.disjointVarSet Core.elemVarSet Core.emptyInScopeSet
+     Core.extendInScopeSet Core.extendInScopeSetList Core.isId Core.isLocalId
+     Core.minusVarSet Core.mkLams Core.mkLets Core.mkVarApps Core.mkVarSet
+     Core.vanillaIdInfo CoreFVs.CoreExprWithFVs CoreFVs.exprFreeVars CoreFVs.freeVars
+     CoreUtils.exprType CoreUtils.extendInScopeSetBind
+     CoreUtils.extendInScopeSetBndrs Data.Bifunctor.second Data.Foldable.all
+     Data.Foldable.any Data.Foldable.elem Data.Foldable.foldr Data.Traversable.forM
+     Data.Tuple.fst Data.Tuple.snd GHC.Base.map GHC.Base.op_z2218U__
+     GHC.Base.op_zgzg__ GHC.Base.op_zgzgze__ GHC.Base.return_ GHC.Err.head
+     GHC.Prim.rightSection GHC.Utils.Monad.State.Strict.State
+     GHC.Utils.Monad.State.Strict.get GHC.Utils.Monad.State.Strict.put
+     GHC.Utils.Monad.State.Strict.runState HsToCoq.DeferredFix.deferredFix2
+     Id.idJoinArity Id.idJoinPointHood Id.isJoinId Id.setIdInfo Outputable.JoinPoint
+     Util.mapSnd
 *)
